a bunch of exploratory work on semantics

Semantics/Gensyn_Semantics.thy
@@ -1,18 +1,60 @@
-theory Gensym_Semantics
-  imports "../Gensym" "../Gensym_Descend"
+theory Gensyn_Semantics
+  imports "../Gensyn" "../Gensyn_Descend"
 begin
 
 (* TODO:
 break this file up into code and spec? *)
 
+fun nosem_base_sem::
+  "('b, 'r, 'g) gensyn \<Rightarrow>
+    'g \<Rightarrow> 
+    'b \<Rightarrow> 
+    childpath \<Rightarrow> 
+    'mstate \<Rightarrow> 
+    childpath option \<Rightarrow>
+    'mstate \<Rightarrow> 
+     bool"
+  where "nosem_base_sem _ _ _ _ _ _ _ = False"
+
+fun nosem_base_sem_exec ::
+  "('b, 'r, 'g) gensyn \<Rightarrow>
+    'g \<Rightarrow> 
+    'b \<Rightarrow> 
+    childpath \<Rightarrow> 
+    'mstate \<Rightarrow> 
+    (childpath option *
+    'mstate) option"
+  where "nosem_base_sem_exec _ _ _ _ _ = None"
+
+fun nosem_rec_sem ::
+  "('b, 'r, 'g) gensyn \<Rightarrow>
+    'g \<Rightarrow> 
+    'r \<Rightarrow> 
+    childpath \<Rightarrow> 
+    'mstate \<Rightarrow> 
+    childpath option \<Rightarrow>
+    'mstate \<Rightarrow> 
+     bool"
+  where "nosem_rec_sem _ _ _ _ _ _ _ = False"
+
+fun nosem_rec_sem_exec ::
+  "('b, 'r, 'g) gensyn \<Rightarrow>
+    'g \<Rightarrow> 
+    'r \<Rightarrow> 
+    childpath \<Rightarrow> 
+    'mstate \<Rightarrow> 
+    (childpath option *
+    'mstate) option"
+  where "nosem_rec_sem_exec _ _ _ _ _ = None"
+
 locale Gensym_Semantics =
   (* fixes/assumes go here *)
   (* NB: these are "small steps" in that they return a new childpath and don't do a full
          execution *)
-  (* TODO: make these parametric in gensym parameters so that
+  (* TODO: make these parametric in gensyn parameters so that
            they can't do weird computations over tree other than
            calculating new childpath? *)
-  fixes base_sem :: "('b, 'r, 'g) gensym \<Rightarrow>
+  fixes base_sem :: "('b, 'r, 'g) gensyn \<Rightarrow>
                       'g \<Rightarrow> 
                       'b \<Rightarrow> 
                       childpath \<Rightarrow> 
@@ -22,7 +64,7 @@ locale Gensym_Semantics =
                       bool"
   (* TODO: should rec_sem take the list component of GRec?
      probably not *)
-  fixes rec_sem :: "('b, 'r, 'g) gensym \<Rightarrow>
+  fixes rec_sem :: "('b, 'r, 'g) gensyn \<Rightarrow>
                     'g \<Rightarrow>
                     'r \<Rightarrow>
                     childpath \<Rightarrow>
@@ -35,8 +77,8 @@ begin
 (* NB this is a big step semantics. sufficient for Ethereum, but perhaps not enough
    for other platforms
    *)
-inductive gensym_sem ::
-  "('b, 'r, 'g) gensym \<Rightarrow>
+inductive gensyn_sem ::
+  "('b, 'r, 'g) gensyn \<Rightarrow>
    childpath \<Rightarrow>
    'mstate \<Rightarrow>
    'mstate \<Rightarrow>
@@ -44,31 +86,31 @@ inductive gensym_sem ::
   "
   where
   "\<And> t cp g b m m' .
-    gensym_get t cp = Some (GBase g b) \<Longrightarrow>
+    gensyn_get t cp = Some (GBase g b) \<Longrightarrow>
     base_sem t g b cp m None m' \<Longrightarrow>
-    gensym_sem t cp m m'"
+    gensyn_sem t cp m m'"
 
 | "\<And> t cp g b m cp' m' m'' .
-    gensym_get t cp = Some (GBase g b) \<Longrightarrow>
+    gensyn_get t cp = Some (GBase g b) \<Longrightarrow>
     base_sem t g b cp m (Some cp') m' \<Longrightarrow>
-    gensym_sem t cp' m' m'' \<Longrightarrow>
-    gensym_sem t cp m m''"
+    gensyn_sem t cp' m' m'' \<Longrightarrow>
+    gensyn_sem t cp m m''"
 
 | "\<And> t cp g r l m m' .
-   gensym_get t cp = Some (GRec g r l) \<Longrightarrow>
+   gensyn_get t cp = Some (GRec g r l) \<Longrightarrow>
    rec_sem t g r cp m None m' \<Longrightarrow>
-   gensym_sem t cp m m'"
+   gensyn_sem t cp m m'"
 
 | "\<And> t cp g r l m cp' m' m'' .
-   gensym_get t cp = Some (GRec g r l) \<Longrightarrow>
+   gensyn_get t cp = Some (GRec g r l) \<Longrightarrow>
    rec_sem t g r cp m (Some cp') m' \<Longrightarrow>
-   gensym_sem t cp' m' m'' \<Longrightarrow>
-   gensym_sem t cp m m''"
+   gensyn_sem t cp' m' m'' \<Longrightarrow>
+   gensyn_sem t cp m m''"
 
 end
 
 locale Gensym_Semantics_Exec =
-  fixes base_sem_exec :: "('b, 'r, 'g) gensym \<Rightarrow>
+  fixes base_sem_exec :: "('b, 'r, 'g) gensyn \<Rightarrow>
                       'g \<Rightarrow> 
                       'b \<Rightarrow> 
                       childpath \<Rightarrow> 
@@ -76,7 +118,7 @@ locale Gensym_Semantics_Exec =
                       (childpath option *
                       'mstate) option"
 
-  fixes rec_sem_exec :: "('b, 'r, 'g) gensym \<Rightarrow>
+  fixes rec_sem_exec :: "('b, 'r, 'g) gensyn \<Rightarrow>
                       'g \<Rightarrow>
                       'r \<Rightarrow>
                       childpath \<Rightarrow>
@@ -88,40 +130,40 @@ begin
 
 (* fueled interpreter for semantics *)
 (* TODO: count down only for backwards jumps? *)
-fun gensym_sem_exec ::
-  "('b, 'r, 'g) gensym \<Rightarrow>
+fun gensyn_sem_exec ::
+  "('b, 'r, 'g) gensyn \<Rightarrow>
    childpath \<Rightarrow>
    'mstate \<Rightarrow>
     nat \<Rightarrow>
    'mstate option" 
   where
-  "gensym_sem_exec t cp m 0 = None"
+  "gensyn_sem_exec t cp m 0 = None"
 
-| "gensym_sem_exec t cp m (Suc n) =
-    (case gensym_get t cp of
+| "gensyn_sem_exec t cp m (Suc n) =
+    (case gensyn_get t cp of
      None \<Rightarrow> None
      | Some (GBase g b) \<Rightarrow>
        (case base_sem_exec t g b cp m of
              None \<Rightarrow> None
              | Some (None, m') \<Rightarrow> Some m'
-             | Some (Some cp', m') \<Rightarrow> gensym_sem_exec t cp' m' n)
+             | Some (Some cp', m') \<Rightarrow> gensyn_sem_exec t cp' m' n)
      | Some (GRec g r l) \<Rightarrow>
         (case rec_sem_exec t g r cp m of
              None \<Rightarrow> None
              | Some (None, m') \<Rightarrow> Some m'
-             | Some (Some cp', m') \<Rightarrow> gensym_sem_exec t cp' m' n))"
+             | Some (Some cp', m') \<Rightarrow> gensyn_sem_exec t cp' m' n))"
 
-lemma gensym_sem_exec_morefuel :
-  assumes H: "gensym_sem_exec t cp m n = Some m'"
+lemma gensyn_sem_exec_morefuel :
+  assumes H: "gensyn_sem_exec t cp m n = Some m'"
   (*assumes Hn' : "n' > n"*)
-  shows "gensym_sem_exec t cp m (Suc n) = Some m'" using H
+  shows "gensyn_sem_exec t cp m (Suc n) = Some m'" using H
 proof(induction n arbitrary: t cp m m')
   case 0
   then show ?case by auto
 next
   case (Suc nx)
   thus ?case
-  proof(cases "gensym_get t cp")
+  proof(cases "gensyn_get t cp")
     case None
     then show ?thesis using Suc by auto
   next
@@ -177,7 +219,7 @@ next
   qed
 qed
 
-definition gsx_base_sem :: "('b, 'r, 'g) gensym \<Rightarrow>
+definition gsx_base_sem :: "('b, 'r, 'g) gensyn \<Rightarrow>
                       'g \<Rightarrow> 
                       'b \<Rightarrow> 
                       childpath \<Rightarrow> 
@@ -189,7 +231,7 @@ definition gsx_base_sem :: "('b, 'r, 'g) gensym \<Rightarrow>
 "gsx_base_sem  =
   (\<lambda> t g b cp m cp' m' . base_sem_exec t g b cp m = Some (cp', m'))"
 
-definition gsx_rec_sem :: "('b, 'r, 'g) gensym \<Rightarrow>
+definition gsx_rec_sem :: "('b, 'r, 'g) gensyn \<Rightarrow>
                     'g \<Rightarrow>
                     'r \<Rightarrow>
                     childpath \<Rightarrow>
@@ -201,63 +243,63 @@ definition gsx_rec_sem :: "('b, 'r, 'g) gensym \<Rightarrow>
 "gsx_rec_sem  =
   (\<lambda>  t g r cp m cp' m' . rec_sem_exec t g r cp m = Some (cp', m'))"
 
-definition gsx_gensym_sem ::
-"('b, 'r, 'g) gensym \<Rightarrow>
+definition gsx_gensyn_sem ::
+"('b, 'r, 'g) gensyn \<Rightarrow>
    childpath \<Rightarrow>
    'mstate \<Rightarrow>
    'mstate \<Rightarrow>
    bool
   "
 where
-"gsx_gensym_sem  =
-  (\<lambda> t cp m m' . \<exists> fuel . gensym_sem_exec t cp m fuel = Some m')"
+"gsx_gensyn_sem  =
+  (\<lambda> t cp m m' . \<exists> fuel . gensyn_sem_exec t cp m fuel = Some m')"
 
 (* standard version of the semantics *)
 interpretation Gensym_Exec_Semantics : Gensym_Semantics
  gsx_base_sem gsx_rec_sem
   done
 
-lemma gensym_exec_eq_l2r :
+lemma gensyn_exec_eq_l2r :
   fixes t cp m m'
-  shows  "Gensym_Exec_Semantics.gensym_sem t cp m m' \<Longrightarrow> gsx_gensym_sem t cp m m'"
-  proof(induction rule: Gensym_Exec_Semantics.gensym_sem.induct)
+  shows  "Gensym_Exec_Semantics.gensyn_sem t cp m m' \<Longrightarrow> gsx_gensyn_sem t cp m m'"
+  proof(induction rule: Gensym_Exec_Semantics.gensyn_sem.induct)
 case (1 t cp g b m m')
   then show ?case
-    apply(simp add: gsx_gensym_sem_def gsx_base_sem_def)
+    apply(simp add: gsx_gensyn_sem_def gsx_base_sem_def)
     apply(rule_tac x = 1 in exI) apply(auto)
     done
 next
 case (2 t cp g b m cp' m' m'')
   then show ?case
-    apply(simp add: gsx_gensym_sem_def gsx_base_sem_def)
+    apply(simp add: gsx_gensyn_sem_def gsx_base_sem_def)
     apply(auto)
     apply(rule_tac x = "Suc fuel" in exI) apply(auto)
     done
 next
   case (3 t cp g r l m m')
   then show ?case
-    apply(simp add: gsx_gensym_sem_def gsx_rec_sem_def)
+    apply(simp add: gsx_gensyn_sem_def gsx_rec_sem_def)
     apply(rule_tac x = 1 in exI) apply(auto)
     done
 next
   case (4 t cp g r l m cp' m' m'')
   then show ?case
-    apply(simp add: gsx_gensym_sem_def gsx_rec_sem_def)
+    apply(simp add: gsx_gensyn_sem_def gsx_rec_sem_def)
     apply(auto)
     apply(rule_tac x = "Suc fuel" in exI) apply(auto)
     done
 qed
 
-lemma gensym_exec_eq_r2l :
+lemma gensyn_exec_eq_r2l :
   fixes fuel
-  shows "\<And> t cp m m'. gensym_sem_exec t cp m (fuel) = Some m' \<Longrightarrow> Gensym_Exec_Semantics.gensym_sem t cp m m'"
+  shows "\<And> t cp m m'. gensyn_sem_exec t cp m (fuel) = Some m' \<Longrightarrow> Gensym_Exec_Semantics.gensyn_sem t cp m m'"
   proof(induction fuel)
     case 0
     then show ?case by auto
   next
     case (Suc fuel)
     then show ?case 
-    proof(cases "gensym_get t cp")
+    proof(cases "gensyn_get t cp")
       case None
       then show ?thesis using Suc by auto
     next
@@ -277,13 +319,13 @@ lemma gensym_exec_eq_r2l :
             then show ?thesis using Some' GBase Some Suc
             proof(cases a'')
               assume None'' : "a'' = None"
-              then show ?thesis using Pair Some' GBase Some Suc Gensym_Semantics.gensym_sem.intros
+              then show ?thesis using Pair Some' GBase Some Suc Gensym_Semantics.gensyn_sem.intros
                 by (auto simp add:gsx_base_sem_def)
             next
               fix a'''
               assume Some'' : "a'' = Some a'''"
               then show ?thesis using Pair Some' GBase Some Suc 
-                    Gensym_Semantics.gensym_sem.intros(2)[of t cp x11 x12 gsx_base_sem]
+                    Gensym_Semantics.gensyn_sem.intros(2)[of t cp x11 x12 gsx_base_sem]
                 by (auto simp add:gsx_base_sem_def)
             qed
           qed
@@ -306,7 +348,7 @@ lemma gensym_exec_eq_r2l :
       proof(cases a'')
         assume None'' : "a'' = None"
         thus ?thesis using GRec Some Suc Some' Pair
-              Gensym_Semantics.gensym_sem.intros gsx_rec_sem_def
+              Gensym_Semantics.gensyn_sem.intros gsx_rec_sem_def
           by auto
 
       next
@@ -314,7 +356,7 @@ lemma gensym_exec_eq_r2l :
         fix a'''
         assume Some'' : "a'' = Some a'''"
         thus ?thesis using GRec Some Suc Some' Pair
-              Gensym_Semantics.gensym_sem.intros(4)[of t cp x21 x22 x23 gsx_rec_sem] gsx_rec_sem_def
+              Gensym_Semantics.gensyn_sem.intros(4)[of t cp x21 x22 x23 gsx_rec_sem] gsx_rec_sem_def
           by auto
       qed
     qed
@@ -327,17 +369,17 @@ qed
 (* OK, we need some kind of lemma that will let us turn (f = g) into (forall x, f x = g x) *)
 interpretation Gensym_Exec_Semantics_Fuel : Gensym_Semantics
  gsx_base_sem gsx_rec_sem
- rewrites Crew : "Gensym_Exec_Semantics.gensym_sem = gsx_gensym_sem"
+ rewrites Crew : "Gensym_Exec_Semantics.gensyn_sem = gsx_gensyn_sem"
 proof(unfold_locales)
-  have Goal : "\<And> t cp m m' . Gensym_Exec_Semantics.gensym_sem t cp m m' = gsx_gensym_sem t cp m m'" 
+  have Goal : "\<And> t cp m m' . Gensym_Exec_Semantics.gensyn_sem t cp m m' = gsx_gensyn_sem t cp m m'" 
   proof - 
     fix t cp m m'
-    show "Gensym_Exec_Semantics.gensym_sem t cp m m' = gsx_gensym_sem t cp m m'"
-      using gensym_exec_eq_l2r
-                             gensym_exec_eq_r2l gsx_gensym_sem_def by auto
+    show "Gensym_Exec_Semantics.gensyn_sem t cp m m' = gsx_gensyn_sem t cp m m'"
+      using gensyn_exec_eq_l2r
+                             gensyn_exec_eq_r2l gsx_gensyn_sem_def by auto
   qed
 
-    thus "Gensym_Exec_Semantics.gensym_sem = gsx_gensym_sem" by blast
+    thus "Gensym_Exec_Semantics.gensyn_sem = gsx_gensyn_sem" by blast
   qed
 
 end
