Syntax/Syn_Elle.thy
@@ -1,0 +1,23 @@
+theory Syn_Elle imports Main "../Syntax_Utils" (*Syn_I*)
+begin
+
+(* Elle syntax *)
+
+(* TODO: do we even need to import Syn_I? *)
+
+type_synonym ('llx, 'ljx, 'ljix, 'xb, 'xa) syn_elle =
+  "'xb + 'llx + 'ljx + 'ljix + 'xa"
+
+type_synonym ('llx, 'ljx, 'ljix, 'xb, 'xa, 'llxo, 'ljxo, 'ljixo) syn_elle_disc =
+  "('xb * ('llx \<Rightarrow> 'llxo) * ('ljx \<Rightarrow> 'ljxo) * ('ljix \<Rightarrow> 'ljixo) * 'xa)"
+
+definition LLab :: "'llx \<Rightarrow> ('llx, 'ljx, 'ljix, 'xb, 'xa) syn_elle" where
+"LLab x = snth2h x"
+
+definition LJmp :: "'ljx \<Rightarrow> ('llx, 'ljx, 'ljix, 'xb, 'xa) syn_elle" where
+"LJmp x = snth3h x"
+
+definition LJmpI :: "'ljix \<Rightarrow> ('llx, 'ljx, 'ljix, 'xb, 'xa) syn_elle" where
+"LJmpI x = snth4h x"
+
+end
