Syntax/Syn_Embelle.thy
@@ -1,0 +1,16 @@
+theory Syn_Embelle imports Main "../Syntax_Utils"
+begin
+(* TODO: Elle extended with arbitrary embedded content
+   idea: semantics need to be proven to never reach this content *)
+
+type_synonym  ('lex, 'xb, 'xa) syn_embelle =
+  "'xb + 'lex + 'xa"
+
+type_synonym ('lex, 'xb, 'xa, 'lexo) syn_embelle_disc =
+  "('xb * ('lex \<Rightarrow> 'lexo) * 'xa)"
+
+      
+definition LEmbed :: "'lex \<Rightarrow> ('lex, 'xa, 'xb) syn_embelle" where
+"LEmbed x = snth2h x"
+
+end
