Syntax/Syn_I.thy
@@ -1,0 +1,24 @@
+theory Syn_I imports "../Syntax_Utils"
+begin
+(* Syntax with instructions *)
+(* This serves as a template for what
+base-case syntax instatiations look like *)
+
+
+type_synonym ('i, 'xb, 'xa) syn_i =
+  "('xb + 'i + 'xa)"
+
+(* there are other discriminator forms, see Alt_Sym.thy.
+   i think this is the one we want... *)
+type_synonym ('i, 'xb, 'xa, 'o) syn_i_disc =
+  "('xb * ('i \<Rightarrow> 'o) * 'xa)"
+
+fun syn_i_cases ::
+  "('i, 'xb, 'xa) syn_i \<Rightarrow> ('i, 'xb \<Rightarrow> 'o, 'xa \<Rightarrow> 'o, 'o) syn_i_disc \<Rightarrow> 'o" where
+  "syn_i_cases s d = disc3 s d"
+
+(* may run into issues with phantom type variables here *)
+definition LInst :: "'i \<Rightarrow> ('i, 'xb, 'xa) syn_i" where
+    "LInst x = snth2h x"
+
+end
