Syntax/Syn_IThenElle.thy
@@ -1,0 +1,59 @@
+theory Syn_IThenElle imports Syn_I Syn_Elle
+begin
+
+(* can we have a plugin for filling in type parameters
+in sequential order? this would be nice *)
+
+(*
+
+we need to establish a convention for what order to list the
+extension-point parameters in.
+
+i think the innermost things should have their extension
+points listed first
+
+however, we might also want to follow the convention that
+outermost xb and xa come last...
+
+new convention: number extension points
+in the order in which they appear (left to right).
+
+i think this convention would actually be confusing though.
+
+*)
+
+(* this is the "flattened" version, so is to be preferred *)
+type_synonym ('lix, 'llx, 'ljx, 'ljix, 'x0, 'x1, 'x2)
+  syn_i_of_elle =
+  "('lix, 'x0, ('llx, 'ljx, 'ljix, 'x1, 'x2) syn_elle) syn_i"
+
+type_synonym ('lix, 'llx, 'ljx, 'ljix, 'x0, 'x1, 'x2)
+  syn_elle_of_i =
+  "('llx, 'ljx, 'ljix, ('lix, 'x0, 'x1) syn_i, 'x2) syn_elle"  
+
+fun syn_i_elle_flatten ::
+"('lix, 'llx, 'ljx, 'ljix, 'x0, 'x1, 'x2)
+    syn_elle_of_i \<Rightarrow>
+   ('lix, 'llx, 'ljx, 'ljix, 'x0, 'x1, 'x2)
+    syn_i_of_elle"
+where
+"syn_i_elle_flatten x = 
+  reassoc3_sum x"
+
+fun syn_i_elle_deflatten ::
+  "('lix, 'llx, 'ljx, 'ljix, 'x0, 'x1, 'x2)
+    syn_i_of_elle \<Rightarrow>
+   ('lix, 'llx, 'ljx, 'ljix, 'x0, 'x1, 'x2)
+    syn_elle_of_i" where
+"syn_i_elle_deflatten x =
+  deassoc3_sum x
+   "
+
+(* note: in general smap may be needed here,
+for more complex representations. in this case, in the
+deflattened version, the nested representation shows up
+in the first slot, so this is not needed*)
+
+(* next up: experiment with writing functions over these representations *)
+
+end
